move higher level defs and lemmas into rsa_ops

otbn_model/spec/vt_ops.dfy
@@ -9,9 +9,7 @@ module vt_ops {
     import opened powers
     import opened congruences
 
-    /* core datatype definions */
-
-    /* registers definions */
+/* registers definions */
 
     type reg_index = uint5
 
@@ -32,7 +30,7 @@ module vt_ops {
 
     type wdrs_t = wdrs : seq<uint256> | |wdrs| == 32 witness *
 
-    /* flags definions */
+/* flags definions */
 
     // datatype flag = CF | MSB | LSB | ZERO
     datatype flags_t = flags_t(cf: bool, msb: bool, lsb: bool, zero: bool)
@@ -57,7 +55,7 @@ module vt_ops {
         if which_group == 0 then fgps.(fg0 := new_flags_t) else fgps.(fg1 := new_flags_t)
     }
 
-    /* memory definions */
+/* memory definions */
 
     type wmem_t = map<int, seq<uint256>>
 
@@ -66,7 +64,7 @@ module vt_ops {
         addr in h
     }
 
-    /* state definions */
+/* state definions */
 
     datatype state = state(
         gprs: gprs_t, // 32-bit registers
@@ -104,191 +102,7 @@ module vt_ops {
         s.ok
     }
 
-    /* instruction definions */
-
-    datatype ins32 =
-        | ADD(xrd: reg32_t, xrs1: reg32_t, xrs2: reg32_t)
-        | ADDI(xrd: reg32_t, xrs1: reg32_t, imm: uint32)
-        | LUI(xrd: reg32_t, imm: uint32)
-        | SUB(xrd: reg32_t, xrs1: reg32_t, xrs2: reg32_t)
-        | AND(xrd: reg32_t, xrs1: reg32_t, xrs2: reg32_t)
-        | ANDI(xrd: reg32_t, xrs1: reg32_t, imm: uint32)
-        | OR(xrd: reg32_t, xrs1: reg32_t, xrs2: reg32_t)
-        | ORI(xrd: reg32_t, xrs1: reg32_t, imm: uint32)
-        | XOR(xrd: reg32_t, xrs1: reg32_t, xrs2: reg32_t)
-        | XORI(xrd: reg32_t, xrs1: reg32_t, imm: uint32)
-        | LW(xrd: reg32_t, xrs1: reg32_t, imm: uint32)
-        | SW(xrs1: reg32_t, xrs2: reg32_t, imm: uint32)
-        | BEQ(xrs1: reg32_t, xrs2: reg32_t, offset: uint32)
-        | BNE(xrs1: reg32_t, xrs2: reg32_t, offset: uint32)
-        | LOOP(grs: reg32_t, bodysize: uint32)
-        | LOOPI(iterations: uint32, bodysize: uint32)
-        | JAL(xrd: reg32_t, offset: uint32)
-        | JALR(xrd: reg32_t, xrs1: reg32_t, offset: uint32)
-        | CSRRS(xrd: reg32_t, csr: reg32_t, xrs2: reg32_t)
-        | CSRRW(xrd: reg32_t, csr: reg32_t, xrs2: reg32_t)
-        | ECALL // TODO
-
-    datatype ins256 =
-        | BN_ADD(wrd: reg256_t, wrs1: reg256_t, wrs2: reg256_t, shift: shift_t, fg: uint1)
-        | BN_ADDC(wrd: reg256_t, wrs1: reg256_t, wrs2: reg256_t, shift: shift_t, fg: uint1)
-        | BN_ADDI(wrd: reg256_t, wrs1: reg256_t, imm: uint256, fg: uint1)
-        | BN_ADDM(wrd: reg256_t, wrs1: reg256_t, wrs2: reg256_t)
-        | BN_MULQACC(zero: bool, wrs1: reg256_t, qwsel1: uint32, wrs2: reg256_t, qwsel2: uint32, shift_qws: uint2)
-        | BN_MULH(wrd: reg256_t, wrs1: reg256_t, hw1: bool, wrs2: reg256_t, hw2: bool)
-        | BN_SUB(wrd: reg256_t, wrs1: reg256_t, wrs2: reg256_t, shift: shift_t, fg: uint1)
-        | BN_SUBB(wrd: reg256_t, wrs1: reg256_t, wrs2: reg256_t, shift: shift_t, fg: uint1)
-        | BN_SUBI(wrd: reg256_t, wrs1: reg256_t, imm: uint256, fg: uint1)
-        | BN_SUBM(wrd: reg256_t, wrs1: reg256_t, wrs2: reg256_t)
-        | BN_AND(wrd: reg256_t, wrs1: reg256_t, wrs2: reg256_t, shift: shift_t)
-        | BN_OR(wrd: reg256_t, wrs1: reg256_t, wrs2: reg256_t, shift: shift_t)
-        | BN_NOT(wrd: reg256_t, wrs1: reg256_t, wrs2: reg256_t, shift: shift_t)
-        | BN_XOR(wrd: reg256_t, wrs1: reg256_t, wrs2: reg256_t, shift: shift_t)
-        | BN_RSHI(wrd: reg256_t, wrs1: reg256_t, wrs2: reg256_t, imm: uint256)
-        | BN_SEL(wrd: reg256_t, wrs1: reg256_t, wrs2: reg256_t, fg: uint1)
-        | BN_CMP(wrs1: reg256_t, wrs2: reg256_t, fg: uint1)
-        | BN_CMPB(wrs1: reg256_t, wrs2: reg256_t, fg: uint1)
-        | BN_LID(grd: reg32_t, grd_inc: bool, offset: uint32, grs: reg32_t, grs_inc: bool)
-        | BN_SID(grs2: reg32_t, grs2_inc: bool, offset: uint32, grs1: reg32_t, grs1_inc: bool)
-        | BN_MOV(wrd: reg256_t, wrs: reg256_t)
-        | BN_MOVR(grd: reg32_t, grd_inc: bool, grs: reg32_t, grs_inc: bool)
-        | BN_WSRRS // TODO
-        | BN_WSRRW // TODO
-
-    predicate eval_ins32(xins: ins32, s: state, r: state)
-    {
-        if !s.ok then
-            !r.ok
-        else
-            r.ok && (valid_state(s) ==> valid_state(r))
-    }
-
-    predicate eval_ins256(wins: ins256, s: state, r: state)
-    {
-        if !s.ok then
-            !r.ok
-        else
-            r.ok && (valid_state(s) ==> valid_state(r))
-    }
-
-    /* control flow definions */
-
-    datatype code =
-        | Ins32(ins: ins32)
-        | Ins256(bn_ins: ins256)
-        | Block(block: codes)
-        | While(whileCond: whileCond, whileBody: code)
-
-    datatype codes = 
-        | CNil
-        | va_CCons(hd: code, tl: codes)
-
-    datatype whileCond = 
-        | RegCond(r: reg32_t)
-        | ImmCond(c: uint32)
-
-    predicate eval_block(block: codes, s: state, r: state)
-    {
-        if block.CNil? then
-            r == s
-        else
-            exists r': state :: eval_code(block.hd, s, r') && eval_block(block.tl, r', r)
-    }
-
-    function eval_cond(s: state, wc: whileCond): nat
-    {
-        match wc 
-            case RegCond(r) => s.eval_reg32(r)
-            case ImmCond(c) => c
-    }
-
-    predicate eval_while(c: code, n: nat, s: state, r: state)
-        decreases c, n
-    {
-        if s.ok then
-            if n == 0 then
-                s == r
-            else
-                exists loop_body_end: state :: eval_code(c, s, loop_body_end)
-                    && eval_while(c, n - 1, loop_body_end, r)
-        else
-            !r.ok
-    }
-
-    predicate eval_code(c: code, s: state, r: state)
-        decreases c, 0
-    {
-        match c
-            case Ins32(ins) => eval_ins32(ins, s, r)
-            case Ins256(ins) => eval_ins256(ins, s, r)
-            case Block(block) => eval_block(block, s, r)
-            //case IfElse(cond, ifT, ifF) => evalIfElse(cond, ifT, ifF, s, r)
-            case While(cond, body) => eval_while(body, eval_cond(s, cond), s, r)
-    }
-
-    /* auxiliary datatype definions */
-
-    datatype uint512_raw = uint512_cons(
-        lh: uint256, uh: uint256, full: uint512)
-
-	type uint512_view_t = num: uint512_raw |
-		&& num.lh == uint512_lh(num.full)
-		&& num.uh == uint512_uh(num.full)
-		witness *
-
-    predicate valid_uint512_view(
-        wdrs: wdrs_t, num: uint512_view_t,
-        li: int, ui: int)
-        requires -1 <= li < BASE_5;
-        requires -1 <= ui < BASE_5;
-    {
-        && (li == NA || wdrs[li] == num.lh)
-        && (ui == NA || wdrs[ui] == num.uh)
-    }
-
-    predicate valid_wdr_view(wdrs: wdrs_t, slice: seq<uint256>, start: nat, len: nat)
-    {   
-        && |slice| == len
-        && start + len <= 32
-        && wdrs[start..start+len] == slice
-    }
-
-    datatype iter_t = iter_cons(base_addr: int, index: nat, buff: seq<uint256>)
-
-    function bn_lid_next_iter(iter: iter_t, inc: bool): iter_t
-    {
-        iter.(index := if inc then iter.index + 1 else iter.index)
-    }
-
-    predicate iter_mapped(iter: iter_t, address: int)
-    {   
-        // we choose to ingore
-        || (address == NA)
-        // address is correct
-        || (address == iter.base_addr + 32 * iter.index)
-    }
-
-    predicate iter_inv(iter: iter_t, wmem: wmem_t, address: int)
-    {
-        var base_addr := iter.base_addr;
-        // base_addr points to a valid buffer
-        && base_addr in wmem
-        // the view is consistent with wmem
-        && wmem[base_addr] == iter.buff
-        // buff does not extend beyond mem limit
-        && base_addr + 32 * |iter.buff| <= DMEM_LIMIT
-        // the index is within bound (or at end)
-        && iter.index <= |iter.buff| != 0
-        // address is correct
-        && iter_mapped(iter, address)
-    }
-
-    predicate iter_safe(iter: iter_t, wmem: wmem_t, address: int)
-    {
-        && iter_inv(iter, wmem, address)
-        // stronger constraint so we can dereference
-        && iter.index < |iter.buff|
-    }
+/* semantics definions (THESE ARE NOT CONNECTED TO BELOW YET) */
 
     function otbn_addc(x: uint256, y: uint256, shift: shift_t, carry: bool) : (uint256, flags_t)
     {
@@ -392,251 +206,189 @@ module vt_ops {
         (concat / pow2(shift_amt)) % BASE_256
     }
 
-    function {:opaque} to_nat(xs: seq<uint256>): nat
+/* instruction definions (THESE ARE NOT CONNECTED TO ABOVE YET) */
+
+    datatype ins32 =
+        | ADD(xrd: reg32_t, xrs1: reg32_t, xrs2: reg32_t)
+        | ADDI(xrd: reg32_t, xrs1: reg32_t, imm: uint32)
+        | LUI(xrd: reg32_t, imm: uint32)
+        | SUB(xrd: reg32_t, xrs1: reg32_t, xrs2: reg32_t)
+        | AND(xrd: reg32_t, xrs1: reg32_t, xrs2: reg32_t)
+        | ANDI(xrd: reg32_t, xrs1: reg32_t, imm: uint32)
+        | OR(xrd: reg32_t, xrs1: reg32_t, xrs2: reg32_t)
+        | ORI(xrd: reg32_t, xrs1: reg32_t, imm: uint32)
+        | XOR(xrd: reg32_t, xrs1: reg32_t, xrs2: reg32_t)
+        | XORI(xrd: reg32_t, xrs1: reg32_t, imm: uint32)
+        | LW(xrd: reg32_t, xrs1: reg32_t, imm: uint32)
+        | SW(xrs1: reg32_t, xrs2: reg32_t, imm: uint32)
+        | BEQ(xrs1: reg32_t, xrs2: reg32_t, offset: uint32)
+        | BNE(xrs1: reg32_t, xrs2: reg32_t, offset: uint32)
+        | LOOP(grs: reg32_t, bodysize: uint32)
+        | LOOPI(iterations: uint32, bodysize: uint32)
+        | JAL(xrd: reg32_t, offset: uint32)
+        | JALR(xrd: reg32_t, xrs1: reg32_t, offset: uint32)
+        | CSRRS(xrd: reg32_t, csr: reg32_t, xrs2: reg32_t)
+        | CSRRW(xrd: reg32_t, csr: reg32_t, xrs2: reg32_t)
+        | ECALL // TODO
+
+    datatype ins256 =
+        | BN_ADD(wrd: reg256_t, wrs1: reg256_t, wrs2: reg256_t, shift: shift_t, fg: uint1)
+        | BN_ADDC(wrd: reg256_t, wrs1: reg256_t, wrs2: reg256_t, shift: shift_t, fg: uint1)
+        | BN_ADDI(wrd: reg256_t, wrs1: reg256_t, imm: uint256, fg: uint1)
+        | BN_ADDM(wrd: reg256_t, wrs1: reg256_t, wrs2: reg256_t)
+        | BN_MULQACC(zero: bool, wrs1: reg256_t, qwsel1: uint32, wrs2: reg256_t, qwsel2: uint32, shift_qws: uint2)
+        | BN_MULH(wrd: reg256_t, wrs1: reg256_t, hw1: bool, wrs2: reg256_t, hw2: bool)
+        | BN_SUB(wrd: reg256_t, wrs1: reg256_t, wrs2: reg256_t, shift: shift_t, fg: uint1)
+        | BN_SUBB(wrd: reg256_t, wrs1: reg256_t, wrs2: reg256_t, shift: shift_t, fg: uint1)
+        | BN_SUBI(wrd: reg256_t, wrs1: reg256_t, imm: uint256, fg: uint1)
+        | BN_SUBM(wrd: reg256_t, wrs1: reg256_t, wrs2: reg256_t)
+        | BN_AND(wrd: reg256_t, wrs1: reg256_t, wrs2: reg256_t, shift: shift_t)
+        | BN_OR(wrd: reg256_t, wrs1: reg256_t, wrs2: reg256_t, shift: shift_t)
+        | BN_NOT(wrd: reg256_t, wrs1: reg256_t, wrs2: reg256_t, shift: shift_t)
+        | BN_XOR(wrd: reg256_t, wrs1: reg256_t, wrs2: reg256_t, shift: shift_t)
+        | BN_RSHI(wrd: reg256_t, wrs1: reg256_t, wrs2: reg256_t, imm: uint256)
+        | BN_SEL(wrd: reg256_t, wrs1: reg256_t, wrs2: reg256_t, fg: uint1)
+        | BN_CMP(wrs1: reg256_t, wrs2: reg256_t, fg: uint1)
+        | BN_CMPB(wrs1: reg256_t, wrs2: reg256_t, fg: uint1)
+        | BN_LID(grd: reg32_t, grd_inc: bool, offset: uint32, grs: reg32_t, grs_inc: bool)
+        | BN_SID(grs2: reg32_t, grs2_inc: bool, offset: uint32, grs1: reg32_t, grs1_inc: bool)
+        | BN_MOV(wrd: reg256_t, wrs: reg256_t)
+        | BN_MOVR(grd: reg32_t, grd_inc: bool, grs: reg32_t, grs_inc: bool)
+        | BN_WSRRS // TODO
+        | BN_WSRRW // TODO
+
+    predicate eval_ins32(xins: ins32, s: state, r: state)
     {
-        if |xs| == 0 then 0
+        if !s.ok then
+            !r.ok
         else
-            var len' := |xs| - 1;
-            to_nat(xs[..len']) + xs[len'] * pow_B256(len')
+            r.ok && (valid_state(s) ==> valid_state(r))
     }
 
-    lemma to_nat_lemma1(xs: seq<uint256>)
-        requires |xs| == 1
-        ensures to_nat(xs) == xs[0]
+    predicate eval_ins256(wins: ins256, s: state, r: state)
     {
-        reveal to_nat();
-        reveal power();
+        if !s.ok then
+            !r.ok
+        else
+            r.ok && (valid_state(s) ==> valid_state(r))
     }
 
-    lemma to_nat_lemma2(xs: seq<uint256>)
-        requires |xs| == 2
-        ensures to_nat(xs) == xs[0] + xs[1] * BASE_256
+/* control flow definions */
+
+    datatype code =
+        | Ins32(ins: ins32)
+        | Ins256(bn_ins: ins256)
+        | Block(block: codes)
+        | While(whileCond: whileCond, whileBody: code)
+
+    datatype codes = 
+        | CNil
+        | va_CCons(hd: code, tl: codes)
+
+    datatype whileCond = 
+        | RegCond(r: reg32_t)
+        | ImmCond(c: uint32)
+
+    predicate eval_block(block: codes, s: state, r: state)
     {
-        reveal to_nat();
-        to_nat_lemma1(xs[..1]);
-        reveal power();
+        if block.CNil? then
+            r == s
+        else
+            exists r': state :: eval_code(block.hd, s, r') && eval_block(block.tl, r', r)
     }
 
-    lemma to_nat_bound_lemma(x: seq<uint256>)
-        ensures to_nat(x) < pow_B256(|x|)
+    function eval_cond(s: state, wc: whileCond): nat
     {
-        if |x| == 0 {
-            reveal to_nat();
-        } else {
-            assume false;
-        }
+        match wc 
+            case RegCond(r) => s.eval_reg32(r)
+            case ImmCond(c) => c
     }
 
-    lemma to_nat_zero_prepend_lemma(xs: seq<uint256>)
-        ensures to_nat([0] + xs) == to_nat(xs) * BASE_256
-
-    lemma to_nat_prefix_lemma(xs: seq<uint256>, i: nat)
-        requires 1 <= i < |xs|;
-        ensures to_nat(xs[..i]) == to_nat(xs[..i-1]) + xs[i-1] * pow_B256(i-1);
+    predicate eval_while(c: code, n: nat, s: state, r: state)
+        decreases c, n
     {
-        assert xs[..i][..i-1] == xs[..i-1];
-        reveal to_nat();
+        if s.ok then
+            if n == 0 then
+                s == r
+            else
+                exists loop_body_end: state :: eval_code(c, s, loop_body_end)
+                    && eval_while(c, n - 1, loop_body_end, r)
+        else
+            !r.ok
     }
 
-    lemma uint512_view_lemma(num: uint512_view_t)
-        ensures num.full
-            == to_nat([num.lh, num.uh])
-            == num.lh + num.uh * BASE_256;
+    predicate eval_code(c: code, s: state, r: state)
+        decreases c, 0
     {
-        reveal uint512_lh();
-        reveal uint512_uh();
-        to_nat_lemma2([num.lh, num.uh]);
+        match c
+            case Ins32(ins) => eval_ins32(ins, s, r)
+            case Ins256(ins) => eval_ins256(ins, s, r)
+            case Block(block) => eval_block(block, s, r)
+            //case IfElse(cond, ifT, ifF) => evalIfElse(cond, ifT, ifF, s, r)
+            case While(cond, body) => eval_while(body, eval_cond(s, cond), s, r)
     }
 
-    lemma to_nat_zero_extend_lemma(xs': seq<uint256>, xs: seq<uint256>) 
-        requires |xs'| < |xs|
-        requires var len' := |xs'|;
-            && xs[..len'] == xs'
-            && xs[len'.. ] == seq(|xs| - len', i => 0)
-        ensures to_nat(xs') == to_nat(xs);
+/* auxiliary definions */
+
+    datatype uint512_raw = uint512_cons(
+        lh: uint256, uh: uint256, full: uint512)
+
+	type uint512_view_t = num: uint512_raw |
+		&& num.lh == uint512_lh(num.full)
+		&& num.uh == uint512_uh(num.full)
+		witness *
+
+    predicate valid_uint512_view(
+        wdrs: wdrs_t, num: uint512_view_t,
+        li: int, ui: int)
+        requires -1 <= li < BASE_5;
+        requires -1 <= ui < BASE_5;
     {
-        var len, len' := |xs|, |xs'|;
-        reveal to_nat();
-        if len != len' + 1 {
-            var len'' := len-1;
-            calc == {
-                to_nat(xs);
-                to_nat(xs[..len'']) + xs[len''] * pow_B256(len'');
-                to_nat(xs[..len'']);
-                { to_nat_zero_extend_lemma(xs', xs[..len'']); }
-                to_nat(xs');
-            }
-        }
+        && (li == NA || wdrs[li] == num.lh)
+        && (ui == NA || wdrs[ui] == num.uh)
     }
 
-    function seq_addc(xs: seq<uint256>, ys: seq<uint256>) : (seq<uint256>, uint1)
-        requires |xs| == |ys|
-        ensures var (zs, cout) := seq_addc(xs, ys);
-            && |zs| == |xs|
+    predicate valid_wdr_view(wdrs: wdrs_t, slice: seq<uint256>, start: nat, len: nat)
+    {   
+        && |slice| == len
+        && start + len <= 32
+        && wdrs[start..start+len] == slice
+    }
+
+    datatype iter_t = iter_cons(base_addr: int, index: nat, buff: seq<uint256>)
+
+    function bn_lid_next_iter(iter: iter_t, inc: bool): iter_t
     {
-        if |xs| == 0 then ([], 0)
-        else 
-            var len' := |xs| - 1;
-            var (zs', cin) := seq_addc(xs[..len'], ys[..len']);
-            var (z, cout) := uint256_addc(xs[len'], ys[len'], cin);
-            (zs' + [z], cout)
+        iter.(index := if inc then iter.index + 1 else iter.index)
     }
 
-    lemma seq_addc_nat_lemma(xs: seq<uint256>, ys: seq<uint256>, zs: seq<uint256>, cout: uint1)
-        requires |xs| == |ys|;
-        requires seq_addc(xs, ys) == (zs, cout);
-        ensures to_nat(xs) + to_nat(ys) == to_nat(zs) + cout * pow_B256(|xs|)
+    predicate iter_mapped(iter: iter_t, address: int)
+    {   
+        // we choose to ingore
+        || (address == NA)
+        // address is correct
+        || (address == iter.base_addr + 32 * iter.index)
+    }
+
+    predicate iter_inv(iter: iter_t, wmem: wmem_t, address: int)
     {
-        reveal to_nat();
-        if |xs| == 0 {
-            reveal power();
-        } else {
-            var len' := |xs| - 1;
-            var (zs', cin) := seq_addc(xs[..len'], ys[..len']);
-            var (z, _) := uint256_addc(xs[len'], ys[len'], cin);
-            assert xs[len'] + ys[len'] + cin == z + cout * BASE_256;
-
-            calc {
-                to_nat(zs);
-                to_nat(zs') + z * pow_B256(len');
-                    { seq_addc_nat_lemma(xs[..len'], ys[..len'], zs', cin); }
-                to_nat(xs[..len']) + to_nat(ys[..len']) - cin * pow_B256(len') + z * pow_B256(len');
-                to_nat(xs[..len']) + to_nat(ys[..len']) + xs[len'] * pow_B256(len') + ys[len'] * pow_B256(len') - cout * BASE_256 * pow_B256(len');
-                    { reveal to_nat(); }
-                to_nat(xs) + to_nat(ys) - cout * BASE_256 * pow_B256(len');
-                    { reveal power(); }
-                to_nat(xs) + to_nat(ys) - cout * pow_B256(|xs|);
-            }
-            assert to_nat(zs) + cout * pow_B256(|xs|) == to_nat(xs) + to_nat(ys);
-        }
+        var base_addr := iter.base_addr;
+        // base_addr points to a valid buffer
+        && base_addr in wmem
+        // the view is consistent with wmem
+        && wmem[base_addr] == iter.buff
+        // buff does not extend beyond mem limit
+        && base_addr + 32 * |iter.buff| <= DMEM_LIMIT
+        // the index is within bound (or at end)
+        && iter.index <= |iter.buff| != 0
+        // address is correct
+        && iter_mapped(iter, address)
     }
 
-    function seq_subb(xs: seq<uint256>, ys: seq<uint256>) : (seq<uint256>, uint1)
-        requires |xs| == |ys|
-        ensures var (zs, bout) := seq_subb(xs, ys);
-            && |zs| == |xs|
-    {
-        if |xs| == 0 then ([], 0)
-        else 
-            var len' := |xs| - 1;
-            var (zs, bin) := seq_subb(xs[..len'], ys[..len']);
-            var (z, bout) := uint256_subb(xs[len'], ys[len'], bin);
-            (zs + [z], bout)
-    }
-
-    lemma seq_subb_nat_lemma(xs: seq<uint256>, ys: seq<uint256>, zs: seq<uint256>, bout: uint1)
-        requires |xs| == |ys|
-        requires seq_subb(xs, ys) == (zs, bout);
-        ensures to_nat(xs) - to_nat(ys) + bout * pow_B256(|xs|) == to_nat(zs)
-    {
-        reveal to_nat();
-        if |xs| == 0 {
-            reveal power();
-        } else {
-            var len' := |xs| - 1;
-            var (zs', bin) := seq_subb(xs[..len'], ys[..len']);
-            var (z, _) := uint256_subb(xs[len'], ys[len'], bin);
-            assert bout * BASE_256 + xs[len'] - bin - ys[len'] == z;
-            
-            calc {
-                to_nat(zs);
-                to_nat(zs') + z * pow_B256(len');
-                    { seq_subb_nat_lemma(xs[..len'], ys[..len'], zs', bin); }
-                to_nat(xs[..len']) - to_nat(ys[..len']) + bin * pow_B256(len') + z * pow_B256(len');
-                to_nat(xs[..len']) - to_nat(ys[..len']) + xs[len'] * pow_B256(len') - ys[len'] * pow_B256(len') + bout * BASE_256 * pow_B256(len');
-                    { reveal to_nat(); }
-                to_nat(xs) - to_nat(ys) + bout * BASE_256 * pow_B256(len');
-                    { reveal power(); }
-                to_nat(xs) - to_nat(ys) + bout * pow_B256(|xs|);
-            }
-        }
-    }
-
-    lemma seq_subb_safe_nat_lemma(xs: seq<uint256>, ys: seq<uint256>)
-        requires |xs| == |ys|
-        requires to_nat(xs) >= to_nat(ys)
-        ensures seq_subb(xs, ys).1 == 0
-    {
-        var (zs, bout) := seq_subb(xs, ys);
-        seq_subb_nat_lemma(xs, ys, zs, bout);
-
-        if bout == 1 {
-            assert to_nat(xs) - to_nat(ys) + pow_B256(|xs|) == to_nat(zs);
-            to_nat_bound_lemma(xs);
-            to_nat_bound_lemma(ys);
-            to_nat_bound_lemma(zs);
-            assert false;
-        }
-    }
-
-   datatype pub_key = pub_key(
-        e: nat, 
-        m: nat,
-        m0d: uint256,
-        B256_INV: nat,
-        R: nat,
-        RR: nat,
-        R_INV: nat)
-
-    predicate pub_key_inv(key: pub_key)
-    {
-        && key.m != 0
-        && cong_B256(key.m0d * key.m, BASE_256-1)
-
-        && cong(BASE_256 * key.B256_INV, 1, key.m)
-
-        && key.R == power(BASE_256, NUM_WORDS)
-
-        && key.RR < key.m
-        && cong(key.RR, key.R * key.R, key.m)
-
-        && key.R_INV == power(key.B256_INV, NUM_WORDS)
-        && cong(key.R_INV * key.R, 1, key.m)
-    }
-
-    datatype mm_vars = mm_vars(
-        x_iter: iter_t,
-        y_iter: iter_t,
-        m_iter: iter_t,
-        rr_iter: iter_t,
-        m0d_iter: iter_t,
-        key: pub_key)
-
-    predicate mm_iter_inv(iter: iter_t, wmem: wmem_t, address: int)
+    predicate iter_safe(iter: iter_t, wmem: wmem_t, address: int)
     {
         && iter_inv(iter, wmem, address)
-        && iter.index == 0
-        && |iter.buff| == NUM_WORDS
-    }
-
-    predicate m0d_iter_inv(iter: iter_t, wmem: wmem_t, address: int)
-    {
-        && iter_inv(iter, wmem, address)
-        && iter.index == 0
-        && |iter.buff| == 1
-    }
-
-    predicate mm_vars_inv(
-        vars: mm_vars,
-        wmem: wmem_t,
-        x_addr: int,
-        y_addr: int,
-        m_addr: int,
-        rr_addr: int,
-        m0d_addr: int)
-    {
-        && pub_key_inv(vars.key)
-
-        && mm_iter_inv(vars.x_iter, wmem, x_addr)
-        && mm_iter_inv(vars.y_iter, wmem, y_addr)
-
-        && mm_iter_inv(vars.m_iter, wmem, m_addr)
-        && to_nat(vars.m_iter.buff) == vars.key.m
-
-        && mm_iter_inv(vars.rr_iter, wmem, rr_addr)
-        && to_nat(vars.rr_iter.buff) == vars.key.RR
-
-        && m0d_iter_inv(vars.m0d_iter, wmem, m0d_addr)
-        && vars.m0d_iter.buff[0] == vars.key.m0d
+        // stronger constraint so we can dereference
+        && iter.index < |iter.buff|
     }
 }
