otbn_model/spec/rsa_ops.dfy
@@ -1,0 +1,263 @@
+include "vt_consts.dfy"
+include "bv_ops.dfy"
+include "vt_ops.dfy"
+include "../lib/powers.dfy"
+include "../lib/congruences.dfy"
+
+module rsa_ops {
+    import opened vt_consts
+    import opened bv_ops
+    import opened vt_ops
+    import opened powers
+    import opened congruences
+
+    function {:opaque} to_nat(xs: seq<uint256>): nat
+    {
+        if |xs| == 0 then 0
+        else
+            var len' := |xs| - 1;
+            to_nat(xs[..len']) + xs[len'] * pow_B256(len')
+    }
+
+    lemma to_nat_lemma1(xs: seq<uint256>)
+        requires |xs| == 1
+        ensures to_nat(xs) == xs[0]
+    {
+        reveal to_nat();
+        reveal power();
+    }
+
+    lemma to_nat_lemma2(xs: seq<uint256>)
+        requires |xs| == 2
+        ensures to_nat(xs) == xs[0] + xs[1] * BASE_256
+    {
+        reveal to_nat();
+        to_nat_lemma1(xs[..1]);
+        reveal power();
+    }
+
+    lemma to_nat_bound_lemma(x: seq<uint256>)
+        ensures to_nat(x) < pow_B256(|x|)
+    {
+        if |x| == 0 {
+            reveal to_nat();
+        } else {
+            assume false;
+        }
+    }
+
+    lemma to_nat_zero_prepend_lemma(xs: seq<uint256>)
+        ensures to_nat([0] + xs) == to_nat(xs) * BASE_256
+
+    lemma to_nat_prefix_lemma(xs: seq<uint256>, i: nat)
+        requires 1 <= i < |xs|;
+        ensures to_nat(xs[..i]) == to_nat(xs[..i-1]) + xs[i-1] * pow_B256(i-1);
+    {
+        assert xs[..i][..i-1] == xs[..i-1];
+        reveal to_nat();
+    }
+
+    lemma uint512_view_lemma(num: uint512_view_t)
+        ensures num.full
+            == to_nat([num.lh, num.uh])
+            == num.lh + num.uh * BASE_256;
+    {
+        reveal uint512_lh();
+        reveal uint512_uh();
+        to_nat_lemma2([num.lh, num.uh]);
+    }
+
+    lemma to_nat_zero_extend_lemma(xs': seq<uint256>, xs: seq<uint256>) 
+        requires |xs'| < |xs|
+        requires var len' := |xs'|;
+            && xs[..len'] == xs'
+            && xs[len'.. ] == seq(|xs| - len', i => 0)
+        ensures to_nat(xs') == to_nat(xs);
+    {
+        var len, len' := |xs|, |xs'|;
+        reveal to_nat();
+        if len != len' + 1 {
+            var len'' := len-1;
+            calc == {
+                to_nat(xs);
+                to_nat(xs[..len'']) + xs[len''] * pow_B256(len'');
+                to_nat(xs[..len'']);
+                { to_nat_zero_extend_lemma(xs', xs[..len'']); }
+                to_nat(xs');
+            }
+        }
+    }
+
+    function seq_addc(xs: seq<uint256>, ys: seq<uint256>) : (seq<uint256>, uint1)
+        requires |xs| == |ys|
+        ensures var (zs, cout) := seq_addc(xs, ys);
+            && |zs| == |xs|
+    {
+        if |xs| == 0 then ([], 0)
+        else 
+            var len' := |xs| - 1;
+            var (zs', cin) := seq_addc(xs[..len'], ys[..len']);
+            var (z, cout) := uint256_addc(xs[len'], ys[len'], cin);
+            (zs' + [z], cout)
+    }
+
+    lemma seq_addc_nat_lemma(xs: seq<uint256>, ys: seq<uint256>, zs: seq<uint256>, cout: uint1)
+        requires |xs| == |ys|;
+        requires seq_addc(xs, ys) == (zs, cout);
+        ensures to_nat(xs) + to_nat(ys) == to_nat(zs) + cout * pow_B256(|xs|)
+    {
+        reveal to_nat();
+        if |xs| == 0 {
+            reveal power();
+        } else {
+            var len' := |xs| - 1;
+            var (zs', cin) := seq_addc(xs[..len'], ys[..len']);
+            var (z, _) := uint256_addc(xs[len'], ys[len'], cin);
+            assert xs[len'] + ys[len'] + cin == z + cout * BASE_256;
+
+            calc {
+                to_nat(zs);
+                to_nat(zs') + z * pow_B256(len');
+                    { seq_addc_nat_lemma(xs[..len'], ys[..len'], zs', cin); }
+                to_nat(xs[..len']) + to_nat(ys[..len']) - cin * pow_B256(len') + z * pow_B256(len');
+                to_nat(xs[..len']) + to_nat(ys[..len']) + xs[len'] * pow_B256(len') 
+                    + ys[len'] * pow_B256(len') - cout * BASE_256 * pow_B256(len');
+                    { reveal to_nat(); }
+                to_nat(xs) + to_nat(ys) - cout * BASE_256 * pow_B256(len');
+                    { reveal power(); }
+                to_nat(xs) + to_nat(ys) - cout * pow_B256(|xs|);
+            }
+            assert to_nat(zs) + cout * pow_B256(|xs|) == to_nat(xs) + to_nat(ys);
+        }
+    }
+
+    function seq_subb(xs: seq<uint256>, ys: seq<uint256>) : (seq<uint256>, uint1)
+        requires |xs| == |ys|
+        ensures var (zs, bout) := seq_subb(xs, ys);
+            && |zs| == |xs|
+    {
+        if |xs| == 0 then ([], 0)
+        else 
+            var len' := |xs| - 1;
+            var (zs, bin) := seq_subb(xs[..len'], ys[..len']);
+            var (z, bout) := uint256_subb(xs[len'], ys[len'], bin);
+            (zs + [z], bout)
+    }
+
+    lemma seq_subb_nat_lemma(xs: seq<uint256>, ys: seq<uint256>, zs: seq<uint256>, bout: uint1)
+        requires |xs| == |ys|
+        requires seq_subb(xs, ys) == (zs, bout);
+        ensures to_nat(xs) - to_nat(ys) + bout * pow_B256(|xs|) == to_nat(zs)
+    {
+        reveal to_nat();
+        if |xs| == 0 {
+            reveal power();
+        } else {
+            var len' := |xs| - 1;
+            var (zs', bin) := seq_subb(xs[..len'], ys[..len']);
+            var (z, _) := uint256_subb(xs[len'], ys[len'], bin);
+            assert bout * BASE_256 + xs[len'] - bin - ys[len'] == z;
+            
+            calc {
+                to_nat(zs);
+                to_nat(zs') + z * pow_B256(len');
+                    { seq_subb_nat_lemma(xs[..len'], ys[..len'], zs', bin); }
+                to_nat(xs[..len']) - to_nat(ys[..len']) + bin * pow_B256(len') + z * pow_B256(len');
+                to_nat(xs[..len']) - to_nat(ys[..len']) + xs[len'] * pow_B256(len')
+                    - ys[len'] * pow_B256(len') + bout * BASE_256 * pow_B256(len');
+                    { reveal to_nat(); }
+                to_nat(xs) - to_nat(ys) + bout * BASE_256 * pow_B256(len');
+                    { reveal power(); }
+                to_nat(xs) - to_nat(ys) + bout * pow_B256(|xs|);
+            }
+        }
+    }
+
+    lemma seq_subb_safe_nat_lemma(xs: seq<uint256>, ys: seq<uint256>)
+        requires |xs| == |ys|
+        requires to_nat(xs) >= to_nat(ys)
+        ensures seq_subb(xs, ys).1 == 0
+    {
+        var (zs, bout) := seq_subb(xs, ys);
+        seq_subb_nat_lemma(xs, ys, zs, bout);
+
+        if bout == 1 {
+            assert to_nat(xs) - to_nat(ys) + pow_B256(|xs|) == to_nat(zs);
+            to_nat_bound_lemma(xs);
+            to_nat_bound_lemma(ys);
+            to_nat_bound_lemma(zs);
+            assert false;
+        }
+    }
+
+   datatype pub_key = pub_key(
+        e: nat, 
+        m: nat,
+        m0d: uint256,
+        B256_INV: nat,
+        R: nat,
+        RR: nat,
+        R_INV: nat)
+
+    predicate pub_key_inv(key: pub_key)
+    {
+        && key.m != 0
+        && cong_B256(key.m0d * key.m, BASE_256-1)
+
+        && cong(BASE_256 * key.B256_INV, 1, key.m)
+
+        && key.R == power(BASE_256, NUM_WORDS)
+
+        && key.RR < key.m
+        && cong(key.RR, key.R * key.R, key.m)
+
+        && key.R_INV == power(key.B256_INV, NUM_WORDS)
+        && cong(key.R_INV * key.R, 1, key.m)
+    }
+
+    datatype mm_vars = mm_vars(
+        x_iter: iter_t,
+        y_iter: iter_t,
+        m_iter: iter_t,
+        rr_iter: iter_t,
+        m0d_iter: iter_t,
+        key: pub_key)
+
+    predicate mm_iter_inv(iter: iter_t, wmem: wmem_t, address: int)
+    {
+        && iter_inv(iter, wmem, address)
+        && iter.index == 0
+        && |iter.buff| == NUM_WORDS
+    }
+
+    predicate m0d_iter_inv(iter: iter_t, wmem: wmem_t, address: int)
+    {
+        && iter_inv(iter, wmem, address)
+        && iter.index == 0
+        && |iter.buff| == 1
+    }
+
+    predicate mm_vars_inv(
+        vars: mm_vars,
+        wmem: wmem_t,
+        x_addr: int,
+        y_addr: int,
+        m_addr: int,
+        rr_addr: int,
+        m0d_addr: int)
+    {
+        && pub_key_inv(vars.key)
+
+        && mm_iter_inv(vars.x_iter, wmem, x_addr)
+        && mm_iter_inv(vars.y_iter, wmem, y_addr)
+
+        && mm_iter_inv(vars.m_iter, wmem, m_addr)
+        && to_nat(vars.m_iter.buff) == vars.key.m
+
+        && mm_iter_inv(vars.rr_iter, wmem, rr_addr)
+        && to_nat(vars.rr_iter.buff) == vars.key.RR
+
+        && m0d_iter_inv(vars.m0d_iter, wmem, m0d_addr)
+        && vars.m0d_iter.buff[0] == vars.key.m0d
+    }
+}
